o

simp_raven_lang/lifting.v
@@ -1,3 +1,4 @@
+From iris.algebra Require Import cmra gmap.
 From iris.program_logic Require Export weakestpre.
 From iris.proofmode Require Import tactics.
 From iris.program_logic Require Import ectx_lifting.
@@ -5,11 +6,11 @@ From iris.program_logic Require Import ectx_lifting.
 (* From iris_simp_lang Require Import heap_lib. *)
 From iris Require Import options.
 From raven_iris.simp_raven_lang Require Import ghost_state.
-From stdpp Require Import gmap.
+From stdpp Require Import gmap list.
 Import uPred.
 Import weakestpre.
 
-
+From stdpp Require Import countable.
 
 Class simpLangG Σ := SimpLangG {
   simpLangG_invG : invGS Σ;
@@ -59,7 +60,7 @@ Section lifting.
     - iNext. iIntros (e2 σ2 efs) "%H Hcred".
       inversion H as [  |  |  |  
         | σ0 stk_id0 stk_frm0 e1 fld e' l0 v0 Hstk_frm0  Hl0 Hv0 
-      |  |  |  |  |  |  ]; subst κ efs σ2 σ0 fld stk_id0 e' e1 e2; simpl; iFrame.
+      |  |  |  |  |  |  |  ]; subst κ efs σ2 σ0 fld stk_id0 e' e1 e2; simpl; iFrame.
       
       assert (l = l0) as Hlsubst. 
         { 
@@ -93,7 +94,96 @@ Section lifting.
   Qed.
 
 
-  (* Lemma wp_assign: similar to wp_heap_wr for the Assign statement *)
+  Lemma stack_upd_valid σ stk_id stk_frm v val:
+    let σ' := update_lvar σ v stk_id val in
+      ● to_stackR (stack σ) ⋅ ◯ to_stackR {[stk_id := stk_frm]} ~~>
+      ● to_stackR (stack σ') ⋅ ◯ to_stackR {[stk_id := {| locals := <[v:=val]> (locals stk_frm) |}]}.
+  Proof.
+    intros σ'.
+    apply auth_update.
+    apply iris.algebra.gmap.gmap_local_update.
+    intros stk_id'.
+    destruct (stack σ !! stk_id') eqn:HstkLookup.
+    - rewrite lookup_fmap. rewrite HstkLookup. simpl.
+    destruct (Z.eqb stk_id stk_id') eqn:Hstkid.
+      + rewrite Z.eqb_eq in Hstkid. subst stk_id'. rewrite lookup_fmap. rewrite lookup_insert. simpl. rewrite lookup_fmap. rewrite lookup_insert. simpl.
+
+  Admitted.
+
+
+  Lemma heap_upd_valid :
+    ∀ fs σ, 
+    let l := fresh_loc (global_heap σ) in
+    let σ' := fold_right 
+        (λ f_v acc ,
+          update_heap acc l f_v.1 f_v.2) 
+      σ fs  in
+    let fs_heap_map := fold_right
+        (λ f_v acc, <[heap_addr_constr l f_v.1:=f_v.2]> acc) 
+      ∅ fs in
+    ● to_heapUR (global_heap σ) ~~> ● to_heapUR (global_heap σ') ⋅ ◯ to_heapUR fs_heap_map.
+  Proof. 
+    induction fs as [ | fs fss IH].
+
+    - intros σ l σ' fs_heap_map. simpl in fs_heap_map. subst fs_heap_map. 
+      (* set (σ' := (fold_left
+        (λ (acc : lang.state) (f_v : fld_name * lang.val), update_heap acc l f_v.1 f_v.2)
+        [] σ0)). *)
+      
+      simpl in σ'. subst σ'. unfold to_heapUR. rewrite fmap_empty. apply  auth_update_alloc. unfold ε. 
+        set (hp1 := (λ v : lang.val, to_heap_cellR v) <$> global_heap σ : gmapUR heap_addr heap_cellR).
+        assert (hp1 = ε ⋅ hp1 ) as H0. { admit. }
+        rewrite -> H0 at 2.
+        assert ((∅ : gmapUR heap_addr heap_cellR) = ε ⋅ (∅ : gmapUR heap_addr heap_cellR)) as H1. { admit. }
+        rewrite H1.
+      apply (op_local_update_discrete hp1 ε ∅).
+      intros. simpl. rewrite left_id. done.
+
+      - intros σ l σ' fs_heap_map. simpl in fs_heap_map.
+       simpl in σ'.
+       specialize (IH σ).
+
+      unfold l in IH.
+      remember (fresh_loc (global_heap σ)) as l0 eqn:Hl.
+
+
+      remember (foldr
+          (λ f_v acc, update_heap acc l0 f_v.1 f_v.2)
+        σ fss
+      ) as σ0 eqn:Hσ.
+
+      remember (foldr
+        (λ f_v acc, <[heap_addr_constr l0 f_v.1:=f_v.2]> acc
+        ) ∅ fss
+      ) as fs_heap_map0 eqn:Hfs.
+
+      subst l.
+
+
+      remember σ' as σ'0 eqn:Hσ'.
+      subst σ'.
+      rewrite <- Hσ in Hσ'.
+
+      remember fs_heap_map as fs_heap_map'0 eqn:Hfs'.
+      subst fs_heap_map.
+      rewrite <- Hfs in Hfs'.
+      subst σ'0.
+      subst fs_heap_map'0.
+      rewrite IH.
+      unfold update_heap. simpl.
+      apply auth_update.
+      unfold to_heapUR at 3 4.
+      rewrite fmap_insert. rewrite fmap_insert.
+      apply alloc_local_update.
+      
+      { admit. }
+      { admit. }
+  Admitted.
+
+
+
+
+
 
   Lemma wp_assign stk_id stk_frm v v' e msk:
     {{{ stack_own[ stk_id, stk_frm] ∗ ⌜expr_step e stk_frm (Val v')⌝}}}
@@ -114,7 +204,7 @@ Section lifting.
     - iNext. iIntros (e2 σ2 efs) "%H Hcred".
       inversion H as [  | 
         σ0 stk_id0 stk_frm0 e1 v0 e0 Hstk_frm0 Hv0 
-      |  |  |  |  |  |  |  |  |  ]; subst κ efs σ2 σ0 v0 e1 e2; simpl. 
+      |  |  |  |  |  |  |  |  |  |  ]; subst κ efs σ2 σ0 v0 e1 e2; simpl. 
       (* iFrame. *)
 
       assert (stk_frm0 = stk_frm) as Hstkfrm_subst. { 
@@ -133,7 +223,7 @@ Section lifting.
            with "Hcomb"
       ) 
           as "Hcomb2".
-      { admit. }
+      { apply stack_upd_valid. }
       iMod "Hcomb2" as "Hcomb".
       iDestruct "Hcomb" as "[Hauth Hfrag]".
       iModIntro. iFrame.
@@ -141,7 +231,218 @@ Section lifting.
       + by iFrame. *)
 
       + iApply "HΦ". by iFrame.
+
+  Qed.
+
+
+  Lemma wp_heap_rd stk_id stk_frm fld e val l x msk q:
+  {{{ stack_own[ stk_id, stk_frm ] ∗ ⌜expr_step e stk_frm (Val (LitLoc l))⌝ ∗ l#fld ↦{q%Qp} val }}}
+      (RTFldRd x e fld stk_id) @ msk
+    {{{RET LitUnit; stack_own[ stk_id, StackFrame (<[x:=val]>stk_frm.(locals))] ∗ l#fld ↦{q%Qp} val}}}.
+  Proof.
+    iIntros (Φ) "[Hstk [%HexprStep HHeap]] HΦ".
+    iApply wp_lift_atomic_base_step_no_fork; first done.
+    iIntros (σ ns κ κs nt) "Hstate".
+    iDestruct "Hstate" as "[Hhp [Hproc Hstack]]".
+    iPoseProof (stack_interp_agreement with "Hstack Hstk") as "%HstkPure".
+    iPoseProof (heap_interp_agreement with "Hhp HHeap") as "%HHeapPure".
+    iSplitR.
+    - unfold base_reducible.
+      iExists [], (RTVal LitUnit), (update_lvar σ x stk_id val), [].
+      iPureIntro.
+      apply (FldRdStep σ stk_id stk_frm x e fld l val); try done.
+
+    - iModIntro. iNext. iIntros (e2 σ2 efs) "%H Hcred".
+      inversion H as [ | | | | | 
+          σ0 stk_id0 stk_frm0 v0 e0 fld0 l0 v2 Hstk_frm0 HexSt HlookUp
+        |  |  |  |  |  |  ]; subst v0 e0 fld0 stk_id0 σ0 κ e2 σ2 efs. simpl. iFrame "Hproc Hhp".
+
+      assert (stk_frm0 = stk_frm) as Hstkfrm_subst. { 
+          rewrite HstkPure in Hstk_frm0.  
+          injection Hstk_frm0 as Hstk_frm0; try done.
+      } subst stk_frm0.
+    
+      assert (LitLoc l = LitLoc l0) as Hlsubst. 
+        { apply (expr_step_val_unique _ _ _ _ HexprStep HexSt). } injection  Hlsubst as Hl. subst l0.
+      (* iModIntro. *)
+
+      assert (val = v2) as Hvalsubst. {
+        rewrite HHeapPure in HlookUp.
+        injection HlookUp as HlookUp; try done.
+      } subst v2.
+
+      iSplitR; try done.
+
+      iCombine "Hstack" "Hstk" as "Hcomb".
+
+      iPoseProof (own_update heap_stack_name 
+          (● to_stackR (stack σ) ⋅ ◯ to_stackR {[stk_id := stk_frm]})
+          (● to_stackR (stack σ') ⋅ ◯ to_stackR {[stk_id := {| locals := <[x:=val]> (locals stk_frm) |}]})
+
+           with "Hcomb"
+      ) 
+          as "Hcomb2".
+      { apply stack_upd_valid. }
+      iMod "Hcomb2" as "Hcomb".
+      iDestruct "Hcomb" as "[Hauth Hfrag]".
+      iModIntro. iFrame.
+      iApply "HΦ". iFrame.
+  Qed.
+
+  Fixpoint field_list_to_iprop lexpr fld_vals : iProp Σ := match fld_vals with
+  | [] => ⌜True⌝
+  | (fld,val) :: fld_vals => ( lexpr#fld ↦{1%Qp}(val)) ∗(field_list_to_iprop lexpr fld_vals)
+  end.
+
+  Lemma wp_alloc stk_id stk_frm fs x msk:
+    {{{ stack_own[ stk_id, stk_frm ] }}}
+      (RTAlloc x fs stk_id) @ msk
+    {{{RET LitUnit; ∃ l: loc, stack_own[ stk_id, StackFrame (<[x:=LitLoc l]>stk_frm.(locals))] ∗ field_list_to_iprop l fs}}}.
+  Proof.
+    iIntros (Φ) "Hstk HΦ".
+    iApply wp_lift_atomic_base_step_no_fork; first done.
+    iIntros (σ ns κ κs nt) "Hstate".
+    iDestruct "Hstate" as "[Hhp [Hproc Hstack]]".
+    iPoseProof (stack_interp_agreement with "Hstack Hstk") as "%HstkPure".
+    iSplitR.
+    - unfold base_reducible.
+        set (l := fresh_loc σ.(global_heap)).
+        set (σ' := (foldr (fun f_v  acc => update_heap acc l (fst f_v) (snd f_v)) σ fs)).
+        set (σ'' := update_lvar σ' x stk_id (LitLoc l)). 
+      iExists [], (RTVal LitUnit), σ'', [].
+      iPureIntro.
+      apply (AllocStep σ stk_id x fs); try done.
+
+    - iModIntro. iNext. iIntros (e2 σ2 efs) "%H Hcred".
+    inversion H as [  |  |  |  |  |  |  |
+        | σ0 stk_id0 x0 fs0
+        |  |  |  ]; subst x0 fs0 stk_id0 σ0 κ e2 σ2 efs; simpl; iFrame.
+        iSplitR; try done.
+
+      iCombine "Hstack" "Hstk" as "Hcomb".
+
+      unfold heap_interp.
+
+      set (fs_map := list_to_map fs : gmap fld_name lang.val).
+      set (fs_heap_map := foldr (λ f_v acc, 
+        <[(heap_addr_constr l f_v.1) := f_v.2]> acc) ∅ fs : gmap heap_addr lang.val).
+
+      iPoseProof (own_update heap_heap_name
+        (● to_heapUR (global_heap σ))
+        (● to_heapUR (global_heap σ') ⋅ (◯  (to_heapUR fs_heap_map ) ))
+        with "Hhp"
+      ) as "HHeapUpd".
+
+      { 
+        
+        apply (heap_upd_valid fs σ).
+      }
+
+      assert ((stack σ) = (stack σ')) as H0. {
+        clear H.
+
+        induction fs.
+        - simpl in σ'. subst σ'. done.
+        - simpl in σ'. 
+        remember (foldr (λ f_v acc, update_heap acc l f_v.1 f_v.2) σ fs) as σ0 eqn:Hσ.
+        unfold σ' in IHfs. rewrite IHfs. subst σ'. unfold update_heap. simpl. done.
+      }
+      rewrite H0.
+
+      iPoseProof (own_update heap_stack_name 
+          (● to_stackR (stack σ') ⋅ ◯ to_stackR {[stk_id := stk_frm]})
+          (● to_stackR (stack σ'') ⋅ ◯ to_stackR {[stk_id := {| locals := <[x:=LitLoc l]> (locals stk_frm) |}]})
+
+           with "Hcomb"
+      )
+          as "Hcomb2".
+      { apply stack_upd_valid. }
+      iMod "Hcomb2" as "Hcomb".
+      iDestruct "Hcomb" as "[Hauth Hfrag]".
+      iDestruct "HHeapUpd" as ">[HHeapUpd HHp2]".
+      iModIntro. iFrame.
+
+      assert (procs σ'' = procs σ) as H1.
+      { clear H H0. subst σ''. simpl. subst σ'. induction fs.
+      - simpl. done.
+      - unfold fs_map in IHfs. simpl. apply IHfs.  }
+
+      rewrite H1. iFrame.
+      iApply "HΦ".
+      iExists l. iFrame.
+
+      clear H H0 H1.
+      iClear "Hcred".
+      iInduction fs as [ | ] "IHfs".
+      + simpl. done.
+      +
+      simpl in fs_heap_map.
+      subst fs_heap_map.
+      simpl.
+      unfold to_heapUR.
+      rewrite fmap_insert.
+
+      rewrite insert_singleton_op. 
+      2 : { 
+        (* uniqueness of fields in f_v *)
+        admit.
+       }
+       rewrite auth_frag_op.
+       iDestruct "HHp2" as "[HHp2 HHp3]".
+       
+       destruct a as [fld val]. simpl. iFrame.
+       iApply "IHfs". iApply "HHp3".
+
   Admitted.
+
+  Lemma wp_seq p q r s1 s2 mask:
+  {{{ p }}} s1 @ mask {{{ RET lang.LitUnit; q }}} -∗
+  {{{ q }}} s2 @ mask {{{ RET lang.LitUnit; r }}} -∗
+
+  {{{ p }}} RTSeq s1 s2 @ mask {{{ RET lang.LitUnit; r }}}.
+  Proof.
+    iIntros "#Hs1 #Hs2".
+    iIntros (Φ). iModIntro. iIntros "Hp HΦ".
+    iApply (wp_bind (fill_item (SeqCtx s2)) _ _ _ _).
+    iApply ("Hs1" with "Hp").
+    iNext. iIntros "Hq".
+    simpl.
+
+    iApply wp_lift_base_step; first done.
+    iIntros (σ ns κ κs nt) "Hstate".
+
+    iDestruct "Hstate" as "[Hhp [Hproc Hstack]]".
+    iApply fupd_mask_intro. { set_unfold. try done. }
+    iIntros "Hemp".
+  
+    iSplitR.
+    - iPureIntro. unfold base_reducible. 
+    exists [], s2, σ, [].
+    apply SeqStep.
+
+    - iModIntro. iIntros (e2 σ2 efs).
+    
+    iIntros "%H Hcred".
+    inversion H as [ | | | | | | | | | | | ]; subst s0 σ0 κ s2 σ2 efs. iFrame.
+    simpl. 
+    iMod "Hemp". iModIntro.
+    iFrame.
+    iApply ("Hs2" with "Hq"). iNext; iFrame.
+  Qed.
+
+  Lemma wp_skip p mask stk_id :
+  {{{ p }}} RTSkipS stk_id @ mask {{{ RET lang.LitUnit; p }}}.
+  Proof.
+    iIntros (Φ) "HP HΦ".
+    iApply wp_lift_atomic_base_step_no_fork; first done.
+    iIntros (σ ns κ κs nt) "Hstate".
+    iSplitR.
+    - unfold base_reducible. iExists [], (RTVal LitUnit), σ, [].
+    iPureIntro. apply RTSkipStep.
+
+    - iModIntro. iNext. iIntros (e2 σ2 efs) "%H Hcred". iModIntro.
+    inversion H; subst σ0 κ e2 σ2 efs. iSplitR; try done. iFrame. simpl. iApply "HΦ". iFrame.
+  Qed.
 
 End lifting.
 
